\documentclass{article}

\usepackage[utf8]{inputenc}
\usepackage{amsmath, amssymb}
\usepackage{enumitem}


\title{CS3SD3 - Assignment 3}
\author{Hien Tu - tun1}


\begin{document}

\maketitle

\section*{Question 7}
\begin{enumerate}[label=(\alph*)]
  \item \begin{enumerate}[label=(\roman*)]
          \item $\neg p \Rightarrow r \equiv \neg (\neg p) \lor r) \equiv p \lor
                r$. Since we have $L(s_0) = \{r\}$, $M, s_0 \vDash \varphi$. We
                have $L(s_2) = \{p, q\}$, so $M, s_2 \vDash \varphi$
          \item Since $r \in L(s_0)$, $r \in L(s_1)$, and we can have path $s_0
                \rightarrow s_1 \rightarrow s_1 \rightarrow s_1 \rightarrow
                \dots$, we know that $M, s_0 \vDash \text{EG } r$. Therefore,
                $M, s_0 \vDash \neg \text{EG } r$ is false. Since $r \not \in
                L(s_2)$, we know that $M, s_0 \vDash \neg \text{EG } r$ is true
                as future also includes present.
          \item Since $t \not \in L(s_0)$, we know that $M, s_0 \vDash
                \text{E}(t \text{ U } q)$ is false. Since $q \in L(s_2)$, we
                know that $q$ already holds in $s_2$, thus, we don't need $t$ to
                hold anymore. Therefore, $M, s_2 \vDash \text{E}(t \text{ U }
                q)$ is true.
          \item Since $q \in L(s_2)$, and we have a path $s_0 \rightarrow s_2
                \rightarrow \dots$, we know $M, s_0 \vDash \text{F } q$ is true.
                Since $q \in L(s_2)$, we also know $M, s_2 \vDash \text{F } q$
                is true since future also includes present.
        \end{enumerate}
  \item LTL: $\text{G}(\text{F } p \land (p \Rightarrow \text{F } s) \land (p \Rightarrow
              \text{F } t))$ \\
        CTL: $\text{AG}(\text{F } p \land
                        \text{AG}(p \Rightarrow \text{AF } s) \land
                        \text{AG}(p \Rightarrow \text{AF } t))$
  \item LTL: $\text{G}(\text{F } q \land \text{F } r \land
                        (q \Rightarrow (\neg\, p \text{ U } r)) \land
                        (q \Rightarrow (t \text{ U } r)))$ \\
        CTL: $\text{AG}(\text{F } q \land \text{F } r) \land
              \text{AG}(q \Rightarrow \text{A}(\neg\, p \text{ U } r)) \land
              \text{AG}(q \Rightarrow \text{A}(t \text{ U } r))$
  \item LTL: $s \vDash \text{G}(\text{F } \varPhi)$ \\
        CTL: $s \vDash \text{AG}(\text{AF } \varPhi)$
  \item LTL: $\text{G}((p \Rightarrow \text{F } q) \Rightarrow 
                        (\neg\, r \text{ U } t))$ \\
        CTL: $\text{AG}((p \Rightarrow \text{F } q) \Rightarrow 
                          \text{A}(\neg\, r \text{ U } t))$
  \item LTL: $\text{G}(\text{F } q \land \text{F } r \land 
                        (q \Rightarrow (\neg\, p \text{ U } r)))$ \\
        CTL: $\text{AG}(\text{F } q \land \text{F } r) \land
              \text{AG}(q \Rightarrow \text{A}(\neg\, p \text{ U } r))$
\end{enumerate}
  
\end{document}

















